ECCA/key_lemmas.v
@@ -4,9 +4,6 @@ Require Export continuations.
 Require Export continuations_lemmas.
 Require Export typing_lemmas.
 
-(* Broken until we fix/extend shifted names *)
-
-(* 
 Lemma Cut (g: env) (K : cont) (N: exp) (A B: exp):
 (Types_cont g K (Cont N A B) ->
 Types g N A ->
@@ -26,7 +23,12 @@ induction 1; auto.
 + inversion IHTypes. auto.
 Qed.
 
-(* Lemma weakening (g : env) (x : name) (N A A' : exp):
+
+(* Broken until we fix/extend shifted names *)
+
+
+(*
+Lemma weakening (g : env) (x : name) (N A A' : exp):
   Types g N A ->
   Types (ctx_cons g x (Assum A')) N A.
 Proof.
